compiler/src/compiler/SeparationLogic.v
@@ -4,6 +4,7 @@ Require Export coqutil.Word.Interface coqutil.Word.Properties.
 Require Export coqutil.Map.Interface coqutil.Map.Properties.
 Require Import coqutil.Tactics.rdelta coqutil.Tactics.destr.
 Require Export coqutil.Z.Lia.
+Require Export coqutil.Datatypes.PropSet.
 Require Export bedrock2.Lift1Prop.
 Require Export bedrock2.Map.Separation.
 Require Export bedrock2.Map.SeparationLogic.
@@ -144,11 +145,119 @@ Ltac cancel_by_tag :=
   constr_eq tagL tagR;
   cancel_seps_at_indices i j.
 
-Section Unique.
+Section Footprint.
   Context {key value} {map : map.map key value} {ok : map.ok map}.
+
+  (* if P allows different footprints, we return the intersection of all possible footprints *)
+  Definition footprint_underapprox(P: map -> Prop): key -> Prop :=
+    fun a => forall m, P m -> exists v, map.get m a = Some v.
+
+  (* if P allows different footprints, we return the union of all possible footprints *)
+  Definition footprint_overapprox(P: map -> Prop): key -> Prop :=
+    fun a => exists m v, P m /\ map.get m a = Some v.
 
   Definition unique_footprint(P: map -> Prop): Prop :=
     forall m1 m2, P m1 -> P m2 -> map.same_domain m1 m2.
+
+  Definition non_contrad(P: map -> Prop): Prop := exists m, P m.
+
+  Lemma footprint_underapprox_subset_overapprox: forall (P: map -> Prop),
+      non_contrad P ->
+      subset (footprint_underapprox P) (footprint_overapprox P).
+  Proof.
+    unfold non_contrad, subset, footprint_underapprox, footprint_overapprox,
+           elem_of.
+    intros.
+    destruct H as [m Pm].
+    firstorder idtac.
+  Qed.
+
+  Lemma footprint_overapprox_subset_underapprox: forall (P: map -> Prop),
+      unique_footprint P ->
+      subset (footprint_overapprox P) (footprint_underapprox P).
+  Proof.
+    unfold unique_footprint, subset, footprint_underapprox, footprint_overapprox,
+           elem_of, map.same_domain, map.sub_domain.
+    intros.
+    destruct H0 as [m' [v [Pm G]]].
+    specialize (H _ _ H1 Pm).
+    destruct H as [S1 S2].
+    eapply S2. eassumption.
+  Qed.
+
+  Lemma footprint_over_equals_underapprox: forall (P: map -> Prop),
+      unique_footprint P ->
+      non_contrad P ->
+      footprint_underapprox P = footprint_overapprox P.
+  Proof.
+    intros.
+    apply iff1ToEq.
+    split.
+    - eapply footprint_underapprox_subset_overapprox. assumption.
+    - eapply footprint_overapprox_subset_underapprox. assumption.
+  Qed.
+
+  (* Given that under normal circumstances, footprint_underapprox is the same as
+     footprint_overapprox (see lemma above), we choose to use footprint_underapprox,
+     because it requires no preconditions for footpr_sep_subset_l/r. *)
+
+  Definition footpr := footprint_underapprox.
+
+  Lemma in_footpr_sep_l: forall (x: key) (P Q: map -> Prop),
+      elem_of x (footpr P) ->
+      elem_of x (footpr (P * Q)%sep).
+  Proof.
+    unfold footpr, footprint_underapprox, sep, elem_of.
+    intros.
+    destruct H0 as [mp [mq [Sp [Pmp Qmq]]]].
+    specialize (H mp Pmp).
+    destruct H as [v G].
+    unfold map.split, map.disjoint in Sp. destruct Sp as [? D]. subst.
+    exists v.
+    rewrite map.get_putmany_dec.
+    destr (map.get mq x).
+    - exfalso. eauto.
+    - assumption.
+  Qed.
+
+  Lemma footpr_sep_subset_l: forall (P Q: map -> Prop) (A: key -> Prop),
+      subset (footpr (sep P Q)) A -> subset (footpr P) A.
+  Proof.
+    unfold subset. eauto using in_footpr_sep_l.
+  Qed.
+
+  Lemma in_footpr_sep_r: forall (x: key) (P Q: map -> Prop),
+      elem_of x (footpr Q) ->
+      elem_of x (footpr (P * Q)%sep).
+  Proof.
+    unfold footpr, footprint_underapprox, sep, elem_of.
+    intros.
+    destruct H0 as [mp [mq [Sp [Pmp Qmq]]]].
+    specialize (H mq Qmq).
+    destruct H as [v G].
+    unfold map.split, map.disjoint in Sp. destruct Sp as [? D]. subst.
+    exists v.
+    rewrite map.get_putmany_dec.
+    destr (map.get mq x).
+    - assumption.
+    - discriminate.
+  Qed.
+
+  Lemma footpr_sep_subset_r: forall (P Q: map -> Prop) (A: key -> Prop),
+      subset (footpr (sep P Q)) A -> subset (footpr Q) A.
+  Proof.
+    unfold subset. eauto using in_footpr_sep_r.
+  Qed.
+
+  Lemma shrink_footpr_subset(P Q R: map -> Prop) (A: key -> Prop)
+      (H1: subset (footpr Q) A)
+      (H2: iff1 Q (P * R)%sep):
+      subset (footpr P) A.
+  Proof.
+    intros.
+    apply iff1ToEq in H2. subst Q.
+    eapply footpr_sep_subset_l. eassumption.
+  Qed.
 
   Lemma same_domain_split: forall m1 m2 m1l m1r m2l m2r,
       map.same_domain m1l m2l ->
@@ -196,4 +305,4 @@ Section Unique.
     eapply same_domain_split; cycle 2; eauto.
   Qed.
 
-End Unique.
+End Footprint.
